\documentclass[11pt,fleqn]{article}
\usepackage{latexsym}
\usepackage{amsmath,amsthm}

\begin{document}
\newcommand{\mbf}[1]{\mbox{{\bfseries #1}}}
\newcommand{\N}{\mbf{N}}
\renewcommand{\O}{\mbf{O}}
\newcommand{\tabfrac}[2]{%
	\setlength{\fboxrule}{0pt}%
	\fbox{$\frac{#1}{#2}$}%
}

\noindent Bill Davis 

\noindent September 24th 2009 

\noindent Homework 3

\begin{enumerate} 

\item[3.4.1]
If $f_{Y}(y) = 4y^3$ then 
\[
P(0 \leq Y \leq \frac{1}{2}) = \int_0^{\frac{1}{2}}4y^3 \,dy = \frac{1}{2}-0 =
\frac{1}{2}
\]

\item[3.4.3]

If $f_{Y}(y) = \frac{3}{2}y^2$, then 
\[
P(| Y-\frac{1}{2} | < \frac{1}{4}) = \int_{\frac{1}{4}}^{\frac{3}{4}}
\frac{3}{2}y^2  \,dy = \frac{1}{2}(\frac{3}{4})^3-\frac{1}{2}(\frac{1}{4})^3 =
\frac{26}{128}
\]

\item[3.4.8]
If $f_Y(y)=\lambda e^{-\lambda y}$ then
\[
F_{Y}(y) = -e^{-\lambda y}
\]

\item[3.5.1]

\begin{tabular}{c c c | c}
\hline
Number of Guess & Payoff & Probabality & $E(X)$ \\
\hline
$<$ 5 & -1\$ & 0.935 & -0.935\\
5 & 2 & 0.0514 & 0.1028 \\
6 & 18 & 0.0115 & 0.207 \\
7 & 180 & 0.0016 & 0.288 \\
8 & 1,300 & 0.000135 & 0.1755 \\
9 & 2,600 & 0.00000612 & 0.015912 \\
10 & 10,000 & 0.000000112 & 0.00112 \\
\hline 
 & & E(X) = & -0.144668 \\

\end{tabular}

\item[3.5.9]
The Expected value is 
\[
\int_0^3 y\frac{1}{9}y^2 \,dy = \frac{1}{36}y^4 = \frac{81}{36} = 2.25
\]
\item[3.5.12]
$f_{Y}(y)$ is a valid pdf for $y \geq 1$ because 
\[
\int_1^\infty \frac{1}{y^2} \,dy = \lim_{y\to\infty}-\frac{1}{y} - -\frac{1}{1}
= 1
\]

However the expected value is infinite because 
\[
\int_1^\infty y\frac{1}{y^2} \,dy = \int_1^\infty \frac{1}{y} \,dy = ln(\infty)
- ln(0) = \infty-1 = \infty
\]
\item[3.5.27]
The expected value is 
\[
\sum_{n=0}^{10}{10 \choose
n}\left(\frac{2}{5}\right)^n\left(\frac{3}{5}\right)^{10-n}(3n-4)  
\]
\[
= -0.0241
-0.0403 + 0.241 + 1.074 + 2.0065 +2.207+1.56+0.721+0.212 +0.0361 +0.0027 
\]
\[
=8
\]
\item[3.6.11]
$f_Y(y) = \lambda e^{-\lambda y}$ then 
\[
E(Y) = \int_0^\infty y \cdot \lambda e^{-\lambda y} \,dy 
\]
Then using integration by parts 
\[
E(Y) = \frac{y}{e^{\lambda y}} - \int \frac{-e^-\lambda y}{\lambda} = 
-\frac{y}{e^{\lambda y}} - \frac{e^{-\lambda y}}{\lambda^2}
\]
this equals $ \frac{1}{\lambda^2}$ when evaluated from $0$ to $\infty$

\[
E(Y^2) = \int_0^\infty y^2 \cdot \lambda e^{-\lambda y} \,dy
\] 

using integration by parts twice on this function yields 

\[
\frac{y^2}{e^{\lambda y}} - \left[ \frac{-2y}{\lambda e^{\lambda y}} - 
\frac{2}{\lambda^2 e^{\lambda y}} \right]
\]

this equals $ \frac{2}{\lambda^2}$ when evaluated from $0$ to $\infty$

The variance is then $ \frac{2}{\lambda^2} -  \frac{1}{\lambda^2} = 
\frac{1}{\lambda^2}$.
\end{enumerate}

\end{document}
